RocqOfRust/revm/revm_interpreter/instructions/simulate/host/extcodecopy.v
@@ -1,7 +1,11 @@
 Require Import simulate.RocqOfRust.
 Require Import alloy_primitives.bytes.links.mod.
+Require Import alloy_primitives.bytes.simulate.mod.
 Require Import alloy_primitives.links.aliases.
+Require Import bytes.simulate.bytes.
 Require Import core.links.array.
+Require Import core.num.simulate.mod.
+Require Import core.simulate.cmp.
 Require Import revm.revm_context_interface.links.host.
 Require Import revm.revm_context_interface.links.journaled_state.
 Require Import revm.revm_context_interface.simulate.host.
@@ -14,6 +18,7 @@ Require Import revm.revm_interpreter.links.interpreter.
 Require Import revm.revm_interpreter.links.instruction_result.
 Require Import revm.revm_interpreter.links.interpreter_types.
 Require Import revm.revm_interpreter.simulate.interpreter_types.
+Require Import ruint.simulate.lib.
 
 Definition extcodecopy
     {WIRE H : Set} `{Link WIRE} `{Link H}
@@ -25,52 +30,45 @@ Definition extcodecopy
     (host : H) :
     Interpreter.t WIRE WIRE_types * H :=
   popn_macro interpreter 4 (fun interpreter => (interpreter, host)) (fun arr interpreter =>
-    let '⟬ address_u256; memory_offset_u256; code_offset_u256; len_u256 ⟭ := arr.(array.value) in
-    let address := Impl_IntoAddress_for_U256.into_address address_u256 in
-    let '(code_opt, host) := IHost.(Host.code) host address in
-    match code_opt with
-    | None =>
-      let control :=
-        IInterpreterTypes.(InterpreterTypes.LoopControl_for_Control).(LoopControl.set_instruction_result)
-          interpreter.(Interpreter.control)
-          instruction_result.InstructionResult.FatalExternalError in
-      (interpreter <| Interpreter.control := control |>, host)
-    | Some code =>
-      as_usize_or_fail_ret_macro interpreter len_u256 None
-        (fun interpreter => (interpreter, host))
-        (fun len interpreter =>
-          let '(code, load) := Impl_Eip7702CodeLoad.into_components code in
-          let spec_id :=
-            IInterpreterTypes.(InterpreterTypes.RuntimeFlag_for_RuntimeFlag).(RuntimeFlag.spec_id)
-              interpreter.(Interpreter.runtime_flag) in
-          gas_or_fail_macro interpreter
-            (calc.extcodecopy_cost spec_id len load)
-            (fun interpreter => (interpreter, host))
-            (fun interpreter =>
-              if i[len] =? 0 then
-                (interpreter, host)
-              else
-                as_usize_or_fail_ret_macro interpreter memory_offset_u256 None
-                  (fun interpreter => (interpreter, host))
-                  (fun memory_offset interpreter =>
-                    let code_offset := as_usize_saturated_macro code_offset_u256 in
-                    resize_memory_macro interpreter memory_offset len
-                      (fun interpreter => (interpreter, host))
-                      (fun interpreter =>
-                        let memory :=
-                          IInterpreterTypes.(InterpreterTypes.MemoryTrait_for_Memory).(MemoryTrait.set_data)
-                            interpreter.(Interpreter.memory)
-                            memory_offset
-                            code_offset
-                            len
-                            code.(Bytes.value).(bytes.Bytes.value) in
-                        (interpreter <| Interpreter.memory := memory |>, host)
-                      )
-                  )
-            )
-        )
-    end
-  ).
+  let '⟬ address; memory_offset; code_offset; len_u256 ⟭ := arr.(array.value) in
+  let address := Impl_IntoAddress_for_U256.into_address address in
+  let '(code_opt, host) := IHost.(Host.code) host address in
+  match code_opt with
+  | None =>
+    let control :=
+      IInterpreterTypes.(InterpreterTypes.LoopControl_for_Control).(LoopControl.set_instruction_result)
+        interpreter.(Interpreter.control)
+        instruction_result.InstructionResult.FatalExternalError in
+    (interpreter <| Interpreter.control := control |>, host)
+  | Some code =>
+
+  as_usize_or_fail_ret_macro interpreter len_u256 None
+    (fun interpreter => (interpreter, host)) (fun len interpreter =>
+  let '(code, load) := Impl_Eip7702CodeLoad.into_components code in
+  let spec_id :=
+    IInterpreterTypes.(InterpreterTypes.RuntimeFlag_for_RuntimeFlag).(RuntimeFlag.spec_id)
+      interpreter.(Interpreter.runtime_flag) in
+  gas_or_fail_macro interpreter (calc.extcodecopy_cost spec_id len load)
+    (fun interpreter => (interpreter, host)) (fun interpreter =>
+  if i[len] =? 0 then
+    (interpreter, host)
+  else
+  as_usize_or_fail_ret_macro interpreter memory_offset None
+    (fun interpreter => (interpreter, host)) (fun memory_offset interpreter =>
+  let code_len := Impl_Bytes.len code.(Bytes.value) in
+  let code_offset := Z.min (i[as_usize_saturated_macro code_offset] mod 2^64) i[code_len] in
+  resize_memory_macro interpreter memory_offset len
+    (fun interpreter => (interpreter, host)) (fun interpreter =>
+
+  let memory :=
+    IInterpreterTypes.(InterpreterTypes.MemoryTrait_for_Memory).(MemoryTrait.set_data)
+      interpreter.(Interpreter.memory)
+      memory_offset
+      code_offset
+      len
+      code.(Bytes.value).(bytes.Bytes.value) in
+  (interpreter <| Interpreter.memory := memory |>, host)
+  )))) end).
 
 Lemma extcodecopy_eq
     {WIRE H : Set} `{Link WIRE} `{Link H}
@@ -98,4 +96,94 @@ Lemma extcodecopy_eq
     )
   }}.
 Proof.
-Admitted.
+Opaque Impl_Eip7702CodeLoad.into_components.
+  with_strategy transparent [run_extcodecopy] unfold extcodecopy, run_extcodecopy; cbn.
+  popn_macro_eq InterpreterTypesEq.
+  match goal with
+  | array : array.t _ _ |- _ =>
+    destruct array as [[address [memory_offset [code_offset [len []]]]]]
+  end.
+  s. {
+    apply Impl_IntoAddress_for_U256.into_address_eq.
+  }
+  s. {
+    apply HostEq.
+  }
+  destruct _.(Host.code) as [[code|] ?host]; cbn. 2: {
+    s. {
+      apply InterpreterTypesEq.
+    }
+    s.
+  }
+  as_usize_or_fail_macro_eq InterpreterTypesEq.
+  s. {
+    apply Impl_Eip7702CodeLoad.into_components_eq.
+  }
+  destruct Impl_Eip7702CodeLoad.into_components as [?code ?load]; cbn.
+  s. {
+    apply InterpreterTypesEq.
+  }
+  s. {
+    apply calc.extcodecopy_cost_eq.
+  }
+  gas_macro_eq idtac.
+  s.
+  destruct (_ =? 0); cbn; [s|].
+  as_usize_or_fail_macro_eq InterpreterTypesEq.
+  eapply Run.Let with (result :=
+    (Output.Success (Z.min
+      (i[as_usize_saturated_macro code_offset] mod 2^64)
+      i[Impl_Bytes.len _.(Bytes.value)] : usize
+    ), _)
+  ). {
+    unfold as_usize_saturated_macro, as_u64_saturated_macro; cbn.
+    s. {
+      s_apply Impl_Uint.as_limbs_eq.
+    }
+    s.
+    destruct (_ && _) in |- *; cbn.
+    { s. {
+        apply Impl_usize.max_eq.
+      }
+      s. {
+        apply simulate.mod.Impl_Deref_for_Bytes.Eq.I.
+      }
+      s. {
+        s_apply Impl_Bytes.len_eq.
+      }
+      s. {
+        apply Impl_Ord_for_usize.toplevel_min_eq.
+      }
+      s.
+    }
+    { s. {
+        apply Impl_u64.max_eq.
+      }
+      s. {
+        apply Impl_usize.max_eq.
+      }
+      s. {
+        apply simulate.mod.Impl_Deref_for_Bytes.Eq.I.
+      }
+      s. {
+        s_apply Impl_Bytes.len_eq.
+      }
+      s. {
+        apply Impl_Ord_for_usize.toplevel_min_eq.
+      }
+      s.
+    }
+  }
+  resize_memory_macro_eq InterpreterTypesEq.
+  s. {
+    apply simulate.mod.Impl_Deref_for_Bytes.Eq.I.
+  }
+  s. {
+    apply Impl_Deref_for_Bytes.Eq.I.
+  }
+  s. {
+    s_apply InterpreterTypesEq.
+  }
+  s; now destruct _.(MemoryTrait.resize).
+Transparent Impl_Eip7702CodeLoad.into_components.
+Qed.
