RocqOfRust/revm/revm_interpreter/instructions/simulate/host/sstore.v
@@ -4,12 +4,18 @@ Require Import core.links.array.
 Require Import revm.revm_context_interface.links.host.
 Require Import revm.revm_context_interface.links.journaled_state.
 Require Import revm.revm_context_interface.simulate.host.
+Require Import revm.revm_interpreter.gas.simulate.calc.
+Require Import revm.revm_interpreter.gas.simulate.constants.
 Require Import revm.revm_interpreter.instructions.links.host.sstore.
 Require Import revm.revm_interpreter.instructions.simulate.macros.
+Require Import revm.revm_interpreter.links.gas.
 Require Import revm.revm_interpreter.links.interpreter.
 Require Import revm.revm_interpreter.links.instruction_result.
 Require Import revm.revm_interpreter.links.interpreter_types.
+Require Import revm.revm_interpreter.simulate.gas.
 Require Import revm.revm_interpreter.simulate.interpreter_types.
+Require Import revm.revm_specification.links.hardfork.
+Require Import revm.revm_specification.simulate.hardfork.
 
 Definition sstore
     {WIRE H : Set} `{Link WIRE} `{Link H}
@@ -20,23 +26,60 @@ Definition sstore
     (interpreter : Interpreter.t WIRE WIRE_types)
     (host : H) :
     Interpreter.t WIRE WIRE_types * H :=
-  let set_fatal (interpreter : Interpreter.t WIRE WIRE_types) :=
+  require_non_staticcall_macro interpreter
+    (fun interpreter => (interpreter, host)) (fun interpreter =>
+
+  popn_macro interpreter 2 (fun interpreter => (interpreter, host)) (fun arr interpreter =>
+  let '⟬ index; value ⟭ := arr.(array.value) in
+  let target :=
+    IInterpreterTypes.(InterpreterTypes.InputsTrait_for_Input).(InputTraits.target_address)
+      interpreter.(Interpreter.input) in
+  let '(result, host) := IHost.(Host.sstore) host target index value in
+  match result with
+  | None =>
     let control :=
       IInterpreterTypes.(InterpreterTypes.LoopControl_for_Control).(LoopControl.set_instruction_result)
         interpreter.(Interpreter.control)
         instruction_result.InstructionResult.FatalExternalError in
-    interpreter <| Interpreter.control := control |> in
-  popn_macro interpreter 2 (fun interpreter => (interpreter, host)) (fun arr interpreter =>
-    let '⟬ index; value ⟭ := arr.(array.value) in
-    let target :=
-      IInterpreterTypes.(InterpreterTypes.InputsTrait_for_Input).(InputTraits.target_address)
-        interpreter.(Interpreter.input) in
-    let '(result, host) := IHost.(Host.sstore) host target index value in
-    match result with
-    | Some _ => (interpreter, host)
-    | None => (set_fatal interpreter, host)
-    end
-  ).
+    (interpreter <| Interpreter.control := control |>, host)
+  | Some state_load =>
+
+  let spec_id :=
+    IInterpreterTypes.(InterpreterTypes.RuntimeFlag_for_RuntimeFlag).(RuntimeFlag.spec_id)
+      interpreter.(Interpreter.runtime_flag) in
+  let gas :=
+    IInterpreterTypes.(InterpreterTypes.LoopControl_for_Control).(LoopControl.gas)
+      .(RefStub.projection) interpreter.(Interpreter.control) in
+  if (Impl_SpecId.is_enabled_in spec_id SpecId.ISTANBUL)
+      && (i[gas.(Gas.remaining)] <=? i[constants.CALL_STIPEND]) then
+    let control :=
+      IInterpreterTypes.(InterpreterTypes.LoopControl_for_Control).(LoopControl.set_instruction_result)
+        interpreter.(Interpreter.control)
+        instruction_result.InstructionResult.ReentrancySentryOOG in
+    (interpreter <| Interpreter.control := control |>, host)
+  else
+  let spec_id :=
+    IInterpreterTypes.(InterpreterTypes.RuntimeFlag_for_RuntimeFlag).(RuntimeFlag.spec_id)
+      interpreter.(Interpreter.runtime_flag) in
+  let vals_ref : '& SStoreResult.t :=
+    Ref.immediate Pointer.Kind.Ref state_load.(StateLoad.data) in
+  gas_macro interpreter
+    (calc.sstore_cost spec_id vals_ref state_load.(StateLoad.is_cold))
+    (fun interpreter => (interpreter, host)) (fun interpreter =>
+
+  let spec_id :=
+    IInterpreterTypes.(InterpreterTypes.RuntimeFlag_for_RuntimeFlag).(RuntimeFlag.spec_id)
+      interpreter.(Interpreter.runtime_flag) in
+  let refund := calc.sstore_refund spec_id vals_ref in
+  let gas :=
+    IInterpreterTypes.(InterpreterTypes.LoopControl_for_Control).(LoopControl.gas)
+      .(RefStub.projection) interpreter.(Interpreter.control) in
+  let gas := Impl_Gas.record_refund gas refund in
+  let control :=
+    IInterpreterTypes.(InterpreterTypes.LoopControl_for_Control).(LoopControl.gas)
+      .(RefStub.injection) interpreter.(Interpreter.control) gas in
+  (interpreter <| Interpreter.control := control |>, host))
+  end)).
 
 Lemma sstore_eq
     {WIRE H : Set} `{Link WIRE} `{Link H}
@@ -64,4 +107,80 @@ Lemma sstore_eq
     )
   }}.
 Proof.
-Admitted.
+  with_strategy transparent [run_sstore] unfold sstore, run_sstore; cbn.
+  require_non_staticcall_macro_eq InterpreterTypesEq.
+  popn_macro_eq InterpreterTypesEq.
+  match goal with
+  | arr : array.t aliases.U256.t _ |- _ =>
+    destruct arr as [[index [value []]]]
+  end.
+  s. {
+    apply InterpreterTypesEq.
+  }
+  s. {
+    apply HostEq.
+  }
+  destruct _.(Host.sstore) as [[state_load|] ?host]; cbn. 2: {
+    s. {
+      apply InterpreterTypesEq.
+    }
+    s.
+  }
+  s. {
+    apply InterpreterTypesEq.
+  }
+  s. {
+    apply Impl_SpecId.is_enabled_in_eq.
+  }
+  destruct Impl_SpecId.is_enabled_in; cbn.
+  { s. {
+      apply InterpreterTypesEq.
+    }
+    s. {
+      apply Impl_Gas.remaining_eq.
+    }
+    s.
+    destruct (_ <=? _); cbn.
+    { s. {
+        apply InterpreterTypesEq.
+      }
+      s.
+    }
+    { gas_macro_eq ltac:(
+        s; [apply InterpreterTypesEq|];
+        s; [apply calc.sstore_cost_eq|]
+      ).
+      s. {
+        apply InterpreterTypesEq.
+      }
+      s. {
+        apply InterpreterTypesEq.
+      }
+      s. {
+        apply calc.sstore_refund_eq.
+      }
+      s. {
+        apply Impl_Gas.record_refund_eq.
+      }
+      s.
+    }
+  }
+  { gas_macro_eq ltac:(
+      s; [apply InterpreterTypesEq|];
+      s; [apply calc.sstore_cost_eq|]
+    ).
+    s. {
+      apply InterpreterTypesEq.
+    }
+    s. {
+      apply InterpreterTypesEq.
+    }
+    s. {
+      apply calc.sstore_refund_eq.
+    }
+    s. {
+      apply Impl_Gas.record_refund_eq.
+    }
+    s.
+  }
+Qed.
