RocqOfRust/revm/revm_interpreter/instructions/simulate/system/returndatacopy.v
@@ -1,7 +1,13 @@
 Require Import simulate.RocqOfRust.
+Require Import alloy_primitives.links.aliases.
+Require Import core.links.array.
+Require Import core.slice.simulate.mod.
+Require Import core.num.simulate.mod.
+Require Import revm.revm_interpreter.instructions.simulate.system.memory_resize.
 Require Import revm.revm_interpreter.instructions.links.system.returndatacopy.
 Require Import revm.revm_interpreter.instructions.simulate.macros.
 Require Import revm.revm_specification.links.hardfork.
+Require Import revm.revm_interpreter.links.instruction_result.
 Require Import revm.revm_interpreter.links.interpreter.
 Require Import revm.revm_interpreter.links.interpreter_types.
 Require Import revm.revm_interpreter.simulate.interpreter_types.
@@ -13,10 +19,45 @@ Definition returndatacopy
     (interpreter : Interpreter.t WIRE WIRE_types) :
     Interpreter.t WIRE WIRE_types :=
   check_macro interpreter SpecId.BYZANTIUM id (fun interpreter =>
-    popn_macro interpreter 3
-      id
-      (fun _ interpreter => interpreter)
-  ).
+  popn_macro interpreter 3
+    id (fun arr interpreter =>
+  let '⟬ memory_offset; offset; len ⟭ := arr.(array.value) in
+
+  as_usize_or_fail_macro interpreter len None id (fun len interpreter =>
+  let data_offset := as_usize_saturated_macro offset in
+
+  let data_end := Impl_usize.saturating_add data_offset len in
+  let return_data :=
+    IInterpreterTypes.(InterpreterTypes.ReturnData_for_ReturnData).(ReturnData.buffer)
+      .(RefStub.projection) interpreter.(Interpreter.return_data) in
+  let return_data_len := Impl_Slice.len return_data in
+  let is_eof :=
+    IInterpreterTypes.(InterpreterTypes.RuntimeFlag_for_RuntimeFlag).(RuntimeFlag.is_eof)
+      interpreter.(Interpreter.runtime_flag) in
+  if (i[data_end] >? i[return_data_len]) && negb is_eof then
+    let control :=
+      IInterpreterTypes.(InterpreterTypes.LoopControl_for_Control).(LoopControl.set_instruction_result)
+        interpreter.(Interpreter.control)
+        instruction_result.InstructionResult.OutOfOffset in
+    interpreter <| Interpreter.control := control |>
+  else
+    let '(memory_offset_opt, interpreter) := memory_resize interpreter memory_offset len in
+    match memory_offset_opt with
+    | None => interpreter
+    | Some memory_offset =>
+      let return_data :=
+        IInterpreterTypes.(InterpreterTypes.ReturnData_for_ReturnData).(ReturnData.buffer)
+          .(RefStub.projection) interpreter.(Interpreter.return_data) in
+      let memory :=
+        IInterpreterTypes.(InterpreterTypes.MemoryTrait_for_Memory).(MemoryTrait.set_data)
+          interpreter.(Interpreter.memory)
+          memory_offset
+          data_offset
+          len
+          return_data in
+      interpreter <| Interpreter.memory := memory |>
+    end
+  ))).
 
 Lemma returndatacopy_eq
     {WIRE H : Set} `{Link WIRE} `{Link H}
@@ -38,4 +79,55 @@ Lemma returndatacopy_eq
         [returndatacopy interpreter; host]%stack
       )
     }}.
-Admitted.
+Proof.
+Opaque memory_resize.
+  with_strategy transparent [run_returndatacopy] unfold returndatacopy, run_returndatacopy; cbn.
+  check_macro_eq InterpreterTypesEq.
+  popn_macro_eq InterpreterTypesEq.
+  match goal with
+  | array : array.t aliases.U256.t _ |- _ =>
+    destruct array as [[memory_offset [offset [len []]]]]
+  end.
+  as_usize_or_fail_macro_eq InterpreterTypesEq.
+  eapply Run.Let with (result := (Output.Success (as_usize_saturated_macro offset), _)). {
+    as_usize_saturated_macro_eq.
+  }
+  s. {
+    apply Impl_usize.saturating_add_eq.
+  }
+  (* We explore all the combinations for the `if` *)
+  s. {
+    apply InterpreterTypesEq.
+  }
+  s. {
+    pose proof (Impl_Slice.len_eq (T := u8)) as H_apply.
+    s_apply H_apply.
+  }
+  s.
+  destruct (_ >? _) eqn:H_lt_eq; cbn.
+  { s. {
+      apply InterpreterTypesEq.
+    }
+    s.
+    destruct negb; cbn.
+    Ltac common_end InterpreterTypesEq :=
+      s; [
+        apply memory_resize_eq
+      |];
+      destruct memory_resize as [[?memory_offset|] ?interpreter]; cbn; [|s];
+      s; [
+        apply InterpreterTypesEq
+      |];
+      s; [
+        s_apply InterpreterTypesEq
+      |];
+      s.
+    { s. {
+        apply InterpreterTypesEq.
+      }
+      s.
+    }
+    { common_end InterpreterTypesEq. }
+  }
+  { common_end InterpreterTypesEq. }
+Qed.
